Behavior.thy
@@ -1,5 +1,5 @@
 theory Behavior
-  imports SetsAndMaps Model App ThreadState SystemState DispatchLogic
+  imports SetsAndMaps Model App ThreadState SystemState DispatchLogic RTS
 begin
 
 section \<open>Thread Execution\<close>
@@ -28,67 +28,37 @@ below "lifts" that predicate to an "update" the entire thread state.
 Only the elements @{term vs} and @{term ps} are updated.  
 The other elements of the thread state are unchanged.\<close>
 
-inductive stepInit for a :: "'a App" and t :: "'a ThreadState" where
-  initialize: "appInit a vs ps \<Longrightarrow> stepInit a t (t\<lparr> tvar:= vs, appo:= ps \<rparr>)"
+inductive stepInit for a :: "'a AppBehavior" where
+  initialize: "appInit a ao tvo \<Longrightarrow> stepInit a t (t\<lparr> appo:= ao, tvar:= tvo \<rparr>)"
 
 text \<open>Below a rule inversion property is proved that states that if the
 thread can do a @{term stepInit} step, it must be the case that the
-execution of the thread Initialize entry logic could produce the values
-of the thread variable state and application output port state as
-specified by the Initialize application code transfer "relation" @{term appInit}.\<close>
+execution of the thread Initialize application behavior @{term appInit} could produce the values
+of the thread variable state and application output port state.\<close>
 
 lemma stepInit_ruleinv:
   assumes "stepInit a t t'"
-  shows "appInit a (tvar t') (appo t')"
+  shows "appInit a (appo t') (tvar t')"
 proof -
-  obtain vs ps where h1: "t' = t\<lparr>tvar := vs, appo := ps\<rparr>"
-                 and h2: "appInit a vs ps"
+  obtain ao tvo where h1: "t' = t\<lparr>appo := ao, tvar := tvo\<rparr>"
+                 and h2: "appInit a ao tvo"
     using assms by (metis stepInit.cases)
-  have h3: "vs = tvar t'" using h1
+  have h3: "tvo = tvar t'" using h1
     apply (drule_tac f = tvar in arg_cong)
     by simp
-  have h4: "ps = appo t'" using h1
+  have h4: "ao = appo t'" using h1
     apply (drule_tac f = appo in arg_cong)
     by simp
   thus ?thesis using h2 h3 h4 by blast
 qed
 
-fun receiveInputSrc where
-  "receiveInputSrc pki ps src dst p = (if p \<in> ps then 
-  (case pki p of
-    Data \<Rightarrow> Some (clear (src $ p))
-  | Event \<Rightarrow> Some (tail (src $ p))
-  | EventData \<Rightarrow> Some (clear (src $ p))
-  )
-  else None)"
-
-fun receiveInputDst where
-  "receiveInputDst pki ps src dst p = (if p \<in> ps then
-  (case pki p of
-    Data \<Rightarrow> Some (src $ p )
-  | Event \<Rightarrow> Some (setBuffer (dst $ p) [head (src $ p)] )
-  | EventData \<Rightarrow> Some (clear (dst $ p))
-  )
-  else None)"
-
-inductive receiveInput for pki :: "PortId \<Rightarrow> PortKind"
-                      and ps :: "PortIds"
-                      and src :: "'a PortState"
-                      and dst :: "'a PortState" where
-  default: "receiveInput pki ps src dst 
-              (receiveInputSrc pki ps src dst) 
-              (receiveInputDst pki ps src dst)"
-
-inductive sendOutput for src :: "'a PortState"
-                      and dst :: "'a PortState" where
-  default: "sendOutput src dst (clearAll (dom src) src) src"
 
 (* Computing step *)
 inductive stepThread for cds :: "'a PortState \<Rightarrow> DispatchStatus set"
                 and pki :: "PortId \<Rightarrow> PortKind"
-                and app :: "'a App" (* JH: this provides app "behavior" *)
+                and app :: "'a AppBehavior" 
                 and cat :: "ScheduleState * ScheduleState" (* JH: Stefan says "the state of the control automaton for the thread" *)
-                and t :: "'a ThreadState" where
+                where
   (* Copy to app input ports*)  (* JH: capturing notion of receive input *)
 (* JH: "if there are some values on the infrastructure ports". 
    Stefan says this is a place that we can now improve the formalism by being more 
@@ -100,171 +70,182 @@ inductive stepThread for cds :: "'a PortState \<Rightarrow> DispatchStatus set"
     \<Longrightarrow> stepThread cds pki app cat t (t\<lparr> infi:= infi', appi:= appi', disp:= dsp \<rparr>)"
   (* Compute next state of thread, reading and writing ports *)
   (* Stefan: appi needs to be updated OR all values get overwritten before the next iteration *)
-| compute: "\<lbrakk> cat = (Ready, Running); appCompute app (tvar t) (appi t) (disp t) ws qs \<rbrakk>
-    \<Longrightarrow> stepThread cds pki app cat t (t\<lparr> tvar:= ws, 
-                             appi:= clearAll (dom (appi t)) (appi t), 
-                             appo:= qs \<rparr>)"
+| compute: "\<lbrakk> cat = (Ready, Running); appCompute app (appi t) (tvar t) (disp t) ao tvo \<rbrakk>
+    \<Longrightarrow> stepThread cds pki app cat t (t\<lparr> appi:= clearAll (dom (appi t)) (appi t), 
+                                         appo:= ao,
+                                         tvar:= tvo \<rparr>)"
   (* Copy from app output ports *)
 | complete: "\<lbrakk> cat = (Running, Waiting); sendOutput (appo t) (info t) appo' info' \<rbrakk>
     \<Longrightarrow> stepThread cds pki app cat t (t\<lparr> appo:= appo', info:= info', disp:= DispatchStatus.NotEnabled \<rparr>)"
 
+section \<open>System Execution\<close>
+
 (* Constrain allowed initial states *)
-definition initSys where "initSys m s \<equiv>
-  (isInitializing s) \<and>
-  (\<forall>c ts. inModelCID m c \<and> systemThread s c = Some ts \<longrightarrow> initial_ThreadState m c ts) \<and>
+definition initSys where "initSys bm sc s \<equiv>
+  (wf_SystemState (bmmodel bm) s) \<and>
+  (systemExec s = Initialize (scheduleInit sc)) \<and>
+  (\<forall>c ts. inModelCID (bmmodel bm) c \<and> systemThread s c = Some ts \<longrightarrow> initial_ThreadState (bmmodel bm) c ts) \<and>
   (\<forall>c x. systemState s c = Some x \<longrightarrow> x = Waiting) \<and>
   (systemComms s = {})"
 
-(* System step *)
-inductive stepSys for am :: "'a AppModel"
+(* System initialization step *)
+inductive initStepSys for bm :: "'a BehaviorModel"
                 and cm :: "('u, 'a) Communication"
                 and sc :: "SystemSchedule" (* two schedulers: one for initialisation, one for computation *)
                 (* (substrate state x ports to read), (updated substrate  *)
-                and s :: "('u, 'a) SystemState" where
+                where
   (* Carry out initialization steps while possible *)
   initialize: "\<lbrakk> isInitializing s; systemExec s = Initialize (c#cs);
-                 stepInit (appModelApp am $ c) (systemThread s $ c) t \<rbrakk> \<Longrightarrow> 
-  stepSys am cm sc s (s\<lparr> systemThread:= (systemThread s)(c\<mapsto>t), systemExec:= Initialize cs \<rparr>)"
+                 stepInit (bmbehaviors bm $ c) (systemThread s $ c) t \<rbrakk> \<Longrightarrow> 
+  initStepSys bm cm sc s (s\<lparr> systemThread:= (systemThread s)(c\<mapsto>t), systemExec:= Initialize cs \<rparr>)"
   (* When initialization has terminated, switch to computing phase *)
 | switch: "\<lbrakk> isInitializing s; systemExec s = Initialize []; c \<in> scheduleFirst sc \<rbrakk>
-    \<Longrightarrow> stepSys am cm sc s (s\<lparr> systemPhase:= Computing, systemExec:= Compute c \<rparr>)"
+    \<Longrightarrow> initStepSys bm cm sc s (s\<lparr> systemExec:= Compute c \<rparr>)"
+
+(* System computation step *)
+inductive computeStepSys for bm :: "'a BehaviorModel"
+                and cm :: "('u, 'a) Communication"
+                and sc :: "SystemSchedule" (* two schedulers: one for initialisation, one for computation *)
+                (* (substrate state x ports to read), (updated substrate  *)
+                where
   (* Copy communication into substrate *)
-| push: "\<lbrakk> isComputing s; systemThread s c = Some t; 
-           (sb, it) \<in> comPush cm (systemComms s) (info t) (appModelConns am) \<rbrakk>
-    \<Longrightarrow> stepSys am cm sc s (s\<lparr>
+  push: "\<lbrakk> isComputing s; systemThread s c = Some t; 
+           (sb, it) \<in> comPush cm (systemComms s) (info t) (modelConns (bmmodel bm)) \<rbrakk>
+    \<Longrightarrow> computeStepSys bm cm sc s (s\<lparr>
           systemThread:= (systemThread s)(c\<mapsto>(t\<lparr> info:= it \<rparr>)),
           systemComms:= sb \<rparr>)"
   (* Copy communication from substrate *)
 | pull: "\<lbrakk> isComputing s; systemThread s c = Some t; 
-           (sb, it) \<in> comPull cm (systemComms s) (infi t) (appModelConns am) \<rbrakk> 
-    \<Longrightarrow> stepSys am cm sc s (s\<lparr>
+           (sb, it) \<in> comPull cm (systemComms s) (infi t) (modelConns (bmmodel bm)) \<rbrakk> 
+    \<Longrightarrow> computeStepSys bm cm sc s (s\<lparr>
           systemThread:= (systemThread s)(c\<mapsto>(t\<lparr> infi:= it \<rparr>)),
           systemComms:= sb \<rparr>)"
   (* Execute thread *)
 | execute: "\<lbrakk> isComputing s;
               systemExec s = Compute c;
               c' \<in> scheduleComp sc $ c;
-              stepThread (computeDispatchStatus (appModel am) c) 
-                (appModelPortKind am)
-                (appModelApp am $ c) 
+              stepThread (computeDispatchStatus (bmmodel bm) c) 
+                (bmodelPortKind bm)
+                (bmbehaviors bm $ c) 
                 (systemState s $ c, a) 
                 (systemThread s $ c) t \<rbrakk> 
-    \<Longrightarrow> stepSys am cm sc s (s\<lparr> 
+    \<Longrightarrow> computeStepSys bm cm sc s (s\<lparr> 
           systemThread:= (systemThread s)(c\<mapsto>t), 
           systemState:= (systemState s)(c\<mapsto>a),
           systemExec:= Compute c' \<rparr>)"
 
+lemma compute_not_initialize:
+  assumes comp: "computeStepSys bm cm sc s s'"
+  shows "\<not>isInitializing s"
+  using assms computeStepSys.cases init_not_compute by blast
+
+lemma initialize_not_compute:
+  assumes init: "initStepSys bm cm sc s s'"
+  shows "\<not>isComputing s"
+  using assms initStepSys.simps init_not_compute by blast
+
+definition stepSys where
+  "stepSys bm cm sc s s' \<equiv> initStepSys bm cm sc s s' \<or> computeStepSys bm cm sc s s'"
+
+lemma stepSys_init: "initStepSys bm cm sc s s' \<Longrightarrow> stepSys bm cm sc s s'" by (simp add: stepSys_def)
+
+lemma stepSys_init_rtranclp: "(initStepSys bm cm sc)\<^sup>*\<^sup>* s s' \<Longrightarrow> (stepSys bm cm sc)\<^sup>*\<^sup>* s s'" 
+  by (metis mono_rtranclp stepSys_init)
+
+lemma stepSys_compute: "computeStepSys bm cm sc s s' \<Longrightarrow> stepSys bm cm sc s s'" by (simp add: stepSys_def)
+
+lemma stepSys_compute_rtranclp: "(computeStepSys bm cm sc)\<^sup>*\<^sup>* s s' \<Longrightarrow> (stepSys bm cm sc)\<^sup>*\<^sup>* s s'" 
+  by (metis mono_rtranclp stepSys_compute)
+
+lemma stepSys_initializing:
+  assumes init: "isInitializing s"
+  shows "stepSys bm cm sc s s' = initStepSys bm cm sc s s'"
+  unfolding stepSys_def
+  using compute_not_initialize init by blast
+
+lemma stepSys_initializing_back:
+  assumes init: "isInitializing s'"
+      and step: "stepSys bm cm sc s s'"
+    shows "isInitializing s"
+proof -
+  have "computeStepSys bm cm sc s s' \<Longrightarrow> \<not>isInitializing s'"
+  proof (induction rule: computeStepSys.induct)
+    case (push c t sb it)
+    then show ?case apply simp by fastforce
+  next
+    case (pull c t sb it)
+    then show ?case apply simp by fastforce
+  next
+    case (execute c c' a t)
+    then show ?case by simp
+  qed
+  hence "\<not>computeStepSys bm cm sc s s'" using init by blast
+  hence h2: "initStepSys bm cm sc s s'" using step unfolding stepSys_def by blast
+  thus ?thesis using initStepSys.simps by blast
+qed
+
 lemma stepSysInit_ruleinv:
   assumes init: "isInitializing s"
       and exec: "systemExec s = Initialize (x # xs)"
-      and step: "stepSys am cm sc s s'"
-    shows "stepInit (appModelApp am $ x) (systemThread s $ x) (systemThread s' $ x)"
-proof -
-  have "\<exists>c cs t.
-        s' = s\<lparr>systemThread := (systemThread s)(c\<mapsto>t), systemExec := Initialize cs\<rparr> \<and>
-        isInitializing s \<and>
-        Initialize (x # xs) = Initialize (c # cs) \<and> stepInit (appModelApp am $ c) (systemThread s $ c) t"
-    using exec step by (simp add: stepSys.simps)
-(* old proof
-    apply (erule disjE)
-     apply blast
-    apply (erule disjE)
-    using init apply force
-    using init by force
-*)
-  then obtain c cs t 
-    where h1: "s' = s\<lparr>systemThread := (systemThread s)(c\<mapsto>t), systemExec := Initialize cs\<rparr>"
-      and h2: "systemPhase s = Initializing"
-      and h3: "systemExec s = Initialize (c # cs)"
-      and h4: "stepInit (appModelApp am $ c) (systemThread s $ c) t"
-    using exec isInitializing.elims by blast
-  have h5: "c = x" using exec h3 by force
-  have h6: "t = systemThread s' $ c" by (simp add: h1)
-  show ?thesis
-    using h4 by (simp add: h5 h6)
+      and step: "stepSys bm cm sc s s'"
+    shows "stepInit (bmbehaviors bm $ x) (systemThread s $ x) (systemThread s' $ x)"
+proof - 
+  \<comment> \<open>First show that @{term initStepSys} rule must have been applied, because the
+     @{term Initialize} schedule is not empty.\<close>
+  from assms have h1: "initStepSys bm cm sc s s'" using stepSys_initializing by blast
+  \<comment> \<open>Then the result follows by rule cases.\<close>
+  from init exec h1 show ?thesis using initStepSys.cases by fastforce
 qed
 
 lemma stepSysInit_redsch_ruleinv:
   assumes init: "isInitializing s"
       and exec: "systemExec s = Initialize (x # xs)"
-      and step: "stepSys am cm sc s s'"
+      and step: "stepSys bm cm sc s s'"
     shows "systemExec s' = Initialize xs"
 proof -
-  have "\<exists>c cs t.
-        s' = s\<lparr>systemThread := (systemThread s)(c\<mapsto>t), systemExec := Initialize cs\<rparr> \<and>
-        isInitializing s \<and>
-        Initialize (x # xs) = Initialize (c # cs) \<and> stepInit (appModelApp am $ c) (systemThread s $ c) t"
-    using exec step by (simp add: stepSys.simps)
-(* old proof
-    apply (erule disjE)
-     apply blast
-    apply (erule disjE)
-    using init apply force
-    using init by force
-*)
-  then obtain c cs t 
-    where h1: "s' = s\<lparr>systemThread := (systemThread s)(c\<mapsto>t), systemExec := Initialize cs\<rparr>"
-      and h2: "systemPhase s = Initializing"
-      and h3: "systemExec s = Initialize (c # cs)"
-      and h4: "stepInit (appModelApp am $ c) (systemThread s $ c) t"
-    using exec isInitializing.elims by blast
-  show ?thesis 
-    using exec h1 h3 by fastforce
+  \<comment> \<open>The @{term initStepSys} rule must have been applied, because the
+     @{term Initialize} schedule is not empty.\<close>
+  from assms have h1: "initStepSys bm cm sc s s'" using stepSys_initializing by blast
+  \<comment> \<open>Then the result follows by rule cases.\<close>
+  from init exec h1 show ?thesis using initStepSys.cases by fastforce
 qed
   
 lemma stepSysInit_initInv_ruleinv:
   assumes init: "isInitializing s"
       and exec: "systemExec s = Initialize (x # xs)"
-      and step: "stepSys am cm sc s s'"
+      and step: "stepSys bm cm sc s s'"
     shows "isInitializing s'"
 proof -
-  have "\<exists>c cs t.
-        s' = s\<lparr>systemThread := (systemThread s)(c\<mapsto>t), systemExec := Initialize cs\<rparr> \<and>
-        isInitializing s \<and>
-        Initialize (x # xs) = Initialize (c # cs) \<and> stepInit (appModelApp am $ c) (systemThread s $ c) t"
-    using exec step by (simp add: stepSys.simps)
-(*
-    apply (erule disjE)
-     apply blast
-    apply (erule disjE)
-    using init apply force
-    using init by force
-*)
-  then obtain c cs t 
-    where h1: "s' = s\<lparr>systemThread := (systemThread s)(c\<mapsto>t), systemExec := Initialize cs\<rparr>"
-      and h2: "systemPhase s = Initializing"
-      and h3: "systemExec s = Initialize (c # cs)"
-      and h4: "stepInit (appModelApp am $ c) (systemThread s $ c) t"
-    using exec isInitializing.elims by blast
-  show ?thesis 
-    by (simp add: h1 h2)
+  \<comment> \<open>The @{term initStepSys} rule must have been applied, because the
+     @{term Initialize} schedule is not empty.\<close>
+  from assms have h1: "initStepSys bm cm sc s s'" using stepSys_initializing by blast
+  \<comment> \<open>Then the result follows by rule cases.\<close>
+  from init exec h1 show ?thesis using initStepSys.cases by fastforce
 qed
 
   
 lemma stepSysInit_sc_rev_ruleinv:
-  "\<lbrakk>stepSys am cm sc s s'; systemExec s' = Initialize xs\<rbrakk> \<Longrightarrow> \<exists>x. systemExec s = Initialize (x # xs)"
-proof (induction rule: stepSys.induct)
-  case (initialize c cs t)
-  then show ?case by force
-next
-  case (switch c)
-  then show ?case by simp
-next
-  case (push c t sb it)
-  then show ?case by simp
-next
-  case (pull c t sb it)
-  then show ?case by simp
-next
-  case (execute c c' a t)
-  then show ?case by simp
+  assumes step: "stepSys bm cm sc s s'"
+      and exec: "systemExec s' = Initialize xs"
+    shows "\<exists>x. systemExec s = Initialize (x # xs)"
+proof -
+   \<comment> \<open>Since @{term s'} is initializing, and we took a step, then @{term s} is initializing.\<close>
+  from assms have h1: "isInitializing s" using stepSys_initializing_back init_init by blast
+   \<comment> \<open>We must have taken an init step from @{term s} to @{term s'}.\<close>
+  from assms h1 have h2: "stepSys bm cm sc s s' = initStepSys bm cm sc s s'"
+    using stepSys_initializing by blast
+  from h2 have h3: "initStepSys bm cm sc s s'" using step unfolding stepSys_def by simp
+   \<comment> \<open>..and then the result follows by cases.\<close>
+  from h1 h3 exec show ?thesis using initStepSys.cases by fastforce
 qed
 
 (* Transitive closure of steps; no traces *)
-definition stepsSys where "stepsSys am cm sc = (stepSys am cm sc)\<^sup>*\<^sup>*"
+definition stepsSys where "stepsSys bm cm sc = (stepSys bm cm sc)\<^sup>*\<^sup>*"
+definition initStepsSys where "initStepsSys bm cm sc = (initStepSys bm cm sc)\<^sup>*\<^sup>*"
+definition computeStepsSys where "computeStepsSys bm cm sc = (computeStepSys bm cm sc)\<^sup>*\<^sup>*"
 
 (* Reachable states from allowed initial states *)
-definition reachSys where "reachSys am cm sc y \<equiv> 
-  \<exists>x. initSys (appModel am) x \<and> stepsSys am cm sc x y"
+definition reachSys where "reachSys bm cm sc y \<equiv> 
+  \<exists>x. initSys bm sc x \<and> stepsSys bm cm sc x y"
 
 end
