PortState.thy
@@ -63,20 +63,51 @@ text \<open>A @{term PortState} is well-formed wrt some set of PortIds if its do
    on port state maintain a domain that is aligned with a set of ports
    declared in a component (e.g., all input ports of the component).\<close>
 
-definition wf_PortState_dom :: "'a PortState \<Rightarrow> PortId set \<Rightarrow> bool" where 
-  "wf_PortState_dom ps pids \<equiv> (dom ps) = pids"
+definition wf_PortState_dom :: " PortId set \<Rightarrow> 'a PortState \<Rightarrow> bool" where 
+  "wf_PortState_dom pids ps \<equiv> (dom ps) = pids"
+
 
 text \<open>A @{term PortState} is well-formed if every @{term PortId} in the port state
-is associated with a well-formed @{term Queue} (as defined in Queue.thy).\<close>
+is associated with a well-formed @{term Queue} @{term q} (as defined in Queue.thy)
+and the capacity of the @{term q} is equal to the model-declared size of the
+queue as found in the model @{term PortDescr} @{term pd} .\<close>
 
-definition wf_PortState_queues :: "'a PortState \<Rightarrow> bool" where 
-  "wf_PortState_queues ps \<equiv> \<forall>p \<in> dom ps. wf_Queue (ps $ p)"
+definition wf_PortState_queue :: "Model \<Rightarrow> PortId \<Rightarrow> 'a Queue \<Rightarrow> bool" where
+  "wf_PortState_queue m p q \<equiv> 
+     let pd = (modelPortDescrs m) $ p 
+                in (wf_Queue q \<and> capacity q = size pd)"
+
+text \<open>ToDo: Add well-formedness properties that constrain the strategy 
+fields to match what is in the port descr for the port.\<close>
+
+definition wf_PortState_queues :: "Model \<Rightarrow> PortId set \<Rightarrow> 'a PortState \<Rightarrow> bool" where 
+(* Old definition
+  "wf_PortState_queues m pids ps \<equiv> \<forall>p \<in> dom ps. wf_Queue (ps $ p)" *)
+  "wf_PortState_queues m pids ps \<equiv> 
+    \<forall>p \<in> pids. let q = (ps $ p)  
+                in wf_PortState_queue m p q"
 
 text \<open>The following definition conjoins the well-formedness properties above.\<close>
 
-definition wf_PortState :: "'a PortState \<Rightarrow> PortId set \<Rightarrow> bool" where 
-  "wf_PortState ps pids \<equiv>   wf_PortState_dom ps pids
-                          \<and> wf_PortState_queues ps"
+definition wf_PortState :: "Model \<Rightarrow> PortId set \<Rightarrow> 'a PortState \<Rightarrow> bool" where 
+  "wf_PortState m pids ps  \<equiv>   wf_PortState_dom pids ps
+                             \<and> wf_PortState_queues m pids ps"
+
+text \<open>The following helper lemmas establish properties of elements (queues, buffers)
+that below to well-formed port states.  These are used in proofs that operations
+on port states preserve well-formedness.\<close>
+
+lemma wf_PortState_implies_wf_PortState_queue:
+  assumes wf_ps: "wf_PortState m dom_pids ps"
+  and p_in_dom: "p \<in> dom_pids"
+shows "wf_PortState_queue m p (ps $ p)"
+  using wf_ps p_in_dom
+  by (simp add: wf_PortState_def wf_PortState_queues_def)
+
+
+(*==================================================================
+   O p e r a t i o n s
+ ===================================================================*)
 
 subsection "Operations"
 
@@ -85,6 +116,11 @@ states.  As a naming convention, operations with "PID" in the name
 take a @{term PortId} argument as a reference to a port;
 operations with "PD" in the name to a @{term PortDescr} as a reference
 to a port.\<close>
+
+subsubsection \<open>Accessor Operations\<close>
+
+text \<open>Accessor operators implement queries about the aggregate port state
+or individual ports.  These do not perform logical updates of the port state.\<close>
 
 text \<open>Does port state @{term ps} map port identifier @{term PortId} to some queue?\<close>
 fun portDefinedPID :: "'a PortState \<Rightarrow> PortId \<Rightarrow> bool" 
@@ -107,13 +143,42 @@ text \<open>Does the port state @{term ps} have any queues that have data availa
 fun dataUnavailable :: "'a PortState \<Rightarrow> bool" (* formerly pempty *)
   where "dataUnavailable ps = (\<forall>p \<in> dom ps. \<forall>q. ps p = Some(q) \<longrightarrow> isEmpty q)"
 
-(* ToDo: John: Should reconcile the name of readyPIDs with dataAvailable *)
+(* ToDo: John: Should reconcile the name of readyPIDs with dataAvailablePorts and dataAvailable *)
 
 text \<open>Does the port state @{term ps} have data available on all ports in the
 set @{term pids}?\<close>
 
 fun readyPIDs :: "'a PortState \<Rightarrow> PortId set \<Rightarrow> bool" (* formerly pready *)
   where "readyPIDs ps pids = (\<forall>p \<in> pids. dataAvailablePID ps p)"
+
+text \<open>Return the first value from @{term p}'s queue within port state @{term ps}.\<close>
+
+fun portHeadPID :: "'a PortState \<Rightarrow> PortId \<Rightarrow> 'a"
+  where "portHeadPID ps p = head (ps $ p)"
+
+text \<open>Return the entire buffer of @{term p}'s queue with port state @{term ps}.\<close>
+fun portBufferPID :: "'a PortState \<Rightarrow> PortId \<Rightarrow> 'a list"  
+  where "portBufferPID ps p = buffer (ps $ p)"
+
+subsubsection \<open>Transformer Operations\<close>
+
+text \<open>Transformer operation perform logical updates of the port states.
+Sections that follow will prove well-formedness preservation properties for these.\<close>
+
+text \<open>Transform the port state @{term ps} by replacing @{term p}'s queue
+with queue @{term q}.\<close>
+
+fun portReplacePID :: "'a PortState \<Rightarrow> PortId \<Rightarrow> 'a Queue \<Rightarrow> 'a PortState"
+  where "portReplacePID (ps::'a PortState) p q = ps(p \<mapsto> q)"
+
+text \<open>Transform the port state @{term ps} by replacing @{term p}'s buffer
+with queue @{term b}, leaving the rest of queue (the static properties and error state) unchanged.\<close>
+
+fun portReplaceBufferPID :: "'a PortState \<Rightarrow> PortId \<Rightarrow> 'a list \<Rightarrow> 'a PortState"
+  where "portReplaceBufferPID (ps::'a PortState) p b = 
+    (let q_pre = (ps $ p) in \<comment> \<open>get the current q\<close>
+       let q_post = setBuffer q_pre b in \<comment> \<open>update the queue with a new buffer\<close>
+         ps(p \<mapsto> q_post))"
 
 text \<open>Transform the port state @{term ps} by dequeuing one value from 
 each of the ports in the set @{term pids}?\<close>
@@ -127,24 +192,11 @@ the port @{term p}?\<close>
 fun portDequeuePID :: "'a PortState \<Rightarrow> PortId \<Rightarrow> 'a PortState" 
   where "portDequeuePID ps p = ps(p \<mapsto> tail (ps $ p))"
 
-text \<open>Return the first value from @{term p}'s queue within port state @{term ps}.\<close>
-
-fun portHeadPID :: "'a PortState \<Rightarrow> PortId \<Rightarrow> 'a"
-  where "portHeadPID ps p = head (ps $ p)"
-
-text \<open>Return the entire buffer of @{term p}'s queue with port state @{term ps}.\<close>
-fun portBufferPID :: "'a PortState \<Rightarrow> PortId \<Rightarrow> 'a list"  
-  where "portBufferPID ps p = buffer (ps $ p)"
-
 text \<open>Transform the port state @{term ps} by enqueueing a value @{term v} 
 into @{term p}'s queue.\<close>
 fun portEnqueuePID :: "'a PortState \<Rightarrow> PortId \<Rightarrow> 'a \<Rightarrow> 'a PortState" 
   where "portEnqueuePID ps p v = ps(p \<mapsto> push (ps $ p) v)"
 
-text \<open>Transform the port state @{term ps} by replacing @{term p}'s queue
-with queue @{term q}.\<close>
-fun portReplacePID :: "'a PortState \<Rightarrow> PortId \<Rightarrow> 'a Queue \<Rightarrow> 'a PortState" 
-  where "portReplacePID (ps::'a PortState) p q = ps(p \<mapsto> q)"
 
 text \<open>Transform the port state @{term ps} by clearing 
 all the queue buffers in the set of ports @{term pids}'s.\<close>
@@ -203,55 +255,196 @@ proof -
   by (metis avail fun_upd_triv fun_upd_upd portDefinedPID.elims(2) portDequeuePID.elims portEnqueuePID.elims)
 qed
 
+(*==================================================================
+   O p e r a t i o n    P r o p e r t i e s
+ ===================================================================*)
+
 subsection "Operation Properties"
+
+(*--------------------------
+    R e p l a c e
+  --------------------------*)
 
 subsubsection \<open>@{term portReplacePID} operation preserves well-formedness\<close>
 
-text \<open>If we perform @{term portReplacePID} for port id @{term p} that already exists 
+text \<open>If we perform @{term portReplacePID} for port id @{term p} that exists 
       within port state @{term ps}, 
       then the resulting port state has the same domain.\<close>
 
 lemma portReplacePID_preserves_wf_PortState_dom:
-  assumes wf_ps_dom:   "wf_PortState_dom ps dom_pids" 
+  assumes wf_ps_dom:   "wf_PortState_dom dom_pids ps" 
       and p_in_dom: "p \<in> dom_pids"
-    shows "wf_PortState_dom (portReplacePID ps p q) dom_pids"
+    shows "wf_PortState_dom dom_pids (portReplacePID ps p q) "
 using wf_ps_dom p_in_dom 
   by (auto simp add: wf_PortState_dom_def)
 
+text \<open>If we perform @{term portReplacePID} for port id @{term p} that exists 
+      within well-formed port state @{term ps} and the new queue is also well-formed 
+      with respect to the model, 
+      then the queues in the resulting port state all well-formed
+      with respect to the model.\<close>
+
+lemma portReplacePID_preserves_wf_PortState_queues:
+  assumes wf_ps: "wf_PortState m dom_pids ps"
+      and p_in_dom: "p \<in> dom_pids"
+      and wf_ps_queue: "wf_PortState_queue m p q"
+     shows "wf_PortState_queues m dom_pids (portReplacePID ps p q)"
+  using wf_ps  \<comment> \<open>assume we start with well-formed port states\<close>  
+        p_in_dom 
+        wf_ps_queue \<comment> \<open>assume the new value of the queue is well-formed\<close>
+        wf_PortState_queue_def  \<comment> \<open>well-formedness definitions and associated properties\<close>
+        wf_PortState_queues_def
+        wf_PortState_implies_wf_PortState_queue 
+  by fastforce
+
+
 text \<open>@{term portReplacePID} preserves port state well-formedness.\<close>
 
-lemma pset_preserves_wf_PortState:
-  assumes wf_ps:   "wf_PortState ps dom_pids" 
+lemma portReplacePID_preserves_wf_PortState:
+  assumes wf_ps:   "wf_PortState m dom_pids ps" 
       and p_in_dom: "p \<in> dom_pids"
-      and wf_queue: "wf_Queue q"
-    shows "wf_PortState (portReplacePID ps p q) dom_pids"
-  using wf_ps
-        p_in_dom  
-        portReplacePID_preserves_wf_PortState_dom  
-        wf_PortState_def
-  by (smt (verit) fun_upd_other fun_upd_same map_get_def map_some_val_given portReplacePID.elims 
-     wf_PortState_dom_def wf_PortState_queues_def wf_queue)
+      and wf_ps_queue: "wf_PortState_queue m p q"
+    shows "wf_PortState m dom_pids (portReplacePID ps p q)"
+  using wf_ps \<comment> \<open>assume we start with well-formed port states\<close>
+        p_in_dom 
+        wf_ps_queue \<comment> \<open>assume the new value of the queue is well-formed\<close>
+        portReplacePID_preserves_wf_PortState_dom \<comment> \<open>previous theorems\<close> 
+        portReplacePID_preserves_wf_PortState_queues 
+        wf_PortState_def \<comment> \<open>primary definition\<close>
+     by blast
 
+(*--------------------------
+    R e p l a c e B u f f e r
+  --------------------------*)
 
-subsubsection \<open>@{term portDequeuePID} operation preserves well-formedness\<close>
+subsubsection \<open>@{term portReplaceBufferPID} operation preserves well-formedness\<close>
 
-text \<open>If we perform @{term portDequeuePID} for port id @{term p} that already exists 
+text \<open>If we perform @{term portReplaceBufferPID} for port id @{term p} that exists 
       within port state @{term ps}, 
       then the resulting port state has the same domain.\<close>
 
-lemma pdeq_preserves_wf_PortState_dom: 
-  assumes wf_ps_dom:   "wf_PortState_dom ps dom_pids" 
+lemma portReplaceBufferPID_preserves_wf_PortState_dom:
+  assumes wf_ps_dom:   "wf_PortState_dom dom_pids ps" 
       and p_in_dom: "p \<in> dom_pids"
-    shows "wf_PortState_dom (portDequeuePID ps p) dom_pids"
+    shows "wf_PortState_dom dom_pids (portReplaceBufferPID ps p b) "
+using wf_ps_dom p_in_dom 
+  by (auto simp add: wf_PortState_dom_def)
+
+text \<open>****Update***** If we perform @{term portReplaceBufferPID} for port id @{term p} that exists 
+      within well-formed port state @{term ps} and the new queue is also well-formed 
+      with respect to the model, 
+      then the queues in the resulting port state all well-formed
+      with respect to the model.\<close>
+
+lemma portReplaceBufferPID_preserves_wf_PortState_queues:
+  assumes wf_ps: "wf_PortState m dom_pids ps"
+      and p_in_dom: "p \<in> dom_pids"
+      and b_wf: "length b \<le> (sizePID m p)"
+    shows "wf_PortState_queues m dom_pids (portReplaceBufferPID ps p b)"
+  using wf_ps  \<comment> \<open>assume we start with well-formed port states\<close>  
+        p_in_dom 
+        b_wf \<comment> \<open>assume the new value of the buffer is well-formed\<close>
+        wf_PortState_queue_def  \<comment> \<open>well-formedness definitions and associated properties\<close>
+        wf_PortState_queues_def
+        wf_PortState_implies_wf_PortState_queue 
+        setBuffer_wf \<comment> \<open>setting wf buffer within wf queue produces wf queue\<close>
+  by fastforce
+
+
+text \<open>@{term portReplacePID} preserves port state well-formedness.\<close>
+
+lemma portReplaceBufferPID_preserves_wf_PortState:
+  assumes wf_ps:   "wf_PortState m dom_pids ps" 
+      and p_in_dom: "p \<in> dom_pids"
+      and b_wf: "length b \<le> (sizePID m p)"
+    shows "wf_PortState m dom_pids (portReplaceBufferPID ps p b)"
+  using wf_ps \<comment> \<open>assume we start with well-formed port states\<close>
+        p_in_dom 
+        b_wf \<comment> \<open>assume the new buffer is well-formed wrt queue capacity\<close>
+        portReplaceBufferPID_preserves_wf_PortState_dom \<comment> \<open>previous theorems\<close> 
+        portReplaceBufferPID_preserves_wf_PortState_queues 
+        wf_PortState_def \<comment> \<open>primary definition\<close>
+     by blast
+
+
+(*--------------------------
+    D e q u e u e 
+  --------------------------*)
+
+subsubsection \<open>@{term portDequeuePID} operation preserves well-formedness\<close>
+
+text \<open>If we perform @{term portDequeuePID} for port id @{term p} that exists 
+      within port state @{term ps}, 
+      then the resulting port state has the same domain.\<close>
+
+lemma portDequeuePID_preserves_wf_PortState_dom: 
+  assumes wf_ps_dom:   "wf_PortState_dom dom_pids ps" 
+      and p_in_dom: "p \<in> dom_pids"
+    shows "wf_PortState_dom  dom_pids (portDequeuePID ps p)"
   using wf_ps_dom p_in_dom 
   by (auto simp add: wf_PortState_dom_def)
+
+text \<open>If we perform @{term portDequeuePID} for port id @{term p} that exists 
+      within port state @{term ps}, 
+      then the resulting queue is well-formed.\<close>
+
+lemma portDequeuePID_preserves_wf_PortState_queue:
+  assumes wf_ps: "wf_PortState m dom_pids ps"
+      and p_in_dom: "p \<in> dom_pids"
+    shows "wf_PortState_queue m p ((portDequeuePID ps p) $ p)"
+proof -
+  from wf_ps p_in_dom have wf_operand_queue: "wf_PortState_queue m p (ps $ p)" 
+    by (rule wf_PortState_implies_wf_PortState_queue)
+  show ?thesis
+    using wf_operand_queue (* well-formed input to the dequeue operation *)
+          tail_wf (* properties of tail used in the dequeue operation *)
+          wf_PortState_queue_def  
+       by fastforce 
+    (* ToDo: I'm surprised I don't need the frame conditions on tail to prove this.
+        I would expect something like what is given below
+    using 
+      tail_wf tail_frame_error tail_frame_capacity tail_frame_strategy (* tail properties *)
+      wf_operand_queue (* well-formed input to the dequeue operation *) 
+      wf_PortState_queue_def     *)      
+   qed
+
+text \<open>All the other queues within the port state @{term ps}
+      not operated on by @{term portDequeuePID} are unchanged.\<close>
+
+lemma portDequeuePID_frame:
+  assumes wf_ps: "wf_PortState m dom_pids ps"
+      and p_in_dom: "p \<in> dom_pids"
+    shows "\<forall>p'\<in> dom_pids - {p} .  ((portDequeuePID ps p) $ p') = ps $ p'"
+  by simp
+
+text \<open>If we perform @{term portDequeuePID} for port id @{term p} that exists 
+      within port state @{term ps}, 
+      then all the queues in the resulting port state are well-formed.\<close>
+
+lemma portDequeuePID_preserves_wf_PortState_queues:
+  assumes wf_ps: "wf_PortState m dom_pids ps"
+      and p_in_dom: "p \<in> dom_pids"
+    shows "wf_PortState_queues m dom_pids (portDequeuePID ps p)"
+  using wf_ps \<comment> \<open>assume we start with well-formed port states\<close>
+        wf_PortState_queues_def \<comment> \<open>..which implies that we have well-formed queues\<close>
+        wf_PortState_implies_wf_PortState_queue  \<comment> \<open>..which implies that the argument to dequeue is well-formed\<close>
+        portDequeuePID_preserves_wf_PortState_queue \<comment> \<open>..and dequeue produces a well-formed queue\<close>
+  by fastforce
+
 
 text \<open>@{term portDequeuePID} preserves port state well-formedness.\<close>
 
 lemma pdeq_preserves_wf_PortState: 
- assumes wf_ps:   "wf_PortState ps dom_pids" 
+ assumes wf_ps:   "wf_PortState m dom_pids ps " 
       and p_in_dom: "p \<in> dom_pids"
-    shows "wf_PortState (portDequeuePID ps p) dom_pids"
+    shows "wf_PortState m dom_pids (portDequeuePID ps p)"
+  using wf_ps p_in_dom (* assumptions *)
+        portDequeuePID_preserves_wf_PortState_dom (* lemmas showing subproperties of wf preserved *)
+        portDequeuePID_preserves_wf_PortState_queues 
+        wf_PortState_def (* definition of well-formedness *)
+     by blast
+
+(* old proof
 proof -
   have h1: "dom (portDequeuePID ps p) = dom_pids"
     using p_in_dom wf_ps apply (simp add: wf_PortState_def wf_PortState_dom_def)
@@ -263,4 +456,89 @@ proof -
     apply (simp add: wf_PortState_def wf_PortState_dom_def wf_PortState_queues_def)
     using h1 by force
 qed
+*)
+
+(*--------------------------
+    E n q u e u e
+  --------------------------*)
+
+subsubsection \<open>@{term portEnqueuePID} operation preserves well-formedness\<close>
+
+text \<open>If we perform @{term portEnqueuePID} for port id @{term p} that exists 
+      within port state @{term ps}, 
+      then the resulting port state has the same domain.\<close>
+
+lemma portEnqueuePID_preserves_wf_PortState_dom:
+  assumes wf_ps_dom:   "wf_PortState_dom dom_pids ps" 
+      and p_in_dom: "p \<in> dom_pids"
+    shows "wf_PortState_dom dom_pids (portEnqueuePID ps p v) "
+using wf_ps_dom p_in_dom 
+  by (auto simp add: wf_PortState_dom_def)
+
+text \<open>If we perform @{term portEnqueuePID} for port id @{term p} that exists 
+      within port state @{term ps}, 
+      then the resulting queue is well-formed.\<close>
+
+lemma portEnqueuePID_preserves_wf_PortState_queue:
+  assumes wf_ps: "wf_PortState m dom_pids ps"
+      and p_in_dom: "p \<in> dom_pids"
+    shows "wf_PortState_queue m p ((portEnqueuePID ps p v) $ p)"
+(* ToDo (from John): make this easier to read by introducing names for the old and new queues *)
+proof -
+  from wf_ps p_in_dom have wf_operand_portstate_queue: "wf_PortState_queue m p (ps $ p)" 
+    by (rule wf_PortState_implies_wf_PortState_queue)
+  from p_in_dom wf_operand_portstate_queue
+  have wf_result_push_queue: "wf_Queue (push (ps $ p) v)"
+    using push_wf wf_PortState_queue_def
+    by metis
+  from p_in_dom wf_result_push_queue 
+  have wf_result_queue: "wf_Queue ((portEnqueuePID ps p v) $ p)"
+    using push_wf p_in_dom wf_operand_portstate_queue
+    by simp
+  have capacity_preserved: "capacity ((portEnqueuePID ps p v) $ p) = capacity (ps $ p)"
+    using p_in_dom push_frame_capacity
+    by (metis fun_upd_same map_some_val_given portEnqueuePID.simps) (* ToDo *)
+  from p_in_dom wf_operand_portstate_queue wf_result_queue capacity_preserved
+  show ?thesis
+    by (metis wf_PortState_queue_def)
+qed   
+
+text \<open>If we perform @{term portEnqueuePID} for port id @{term p} that exists 
+      within well-formed port state @{term ps}, 
+      then the queues in the resulting port state all well-formed
+      with respect to the model.\<close>
+
+
+lemma portEnqueuePID_preserves_wf_PortState_queues:
+  assumes wf_ps: "wf_PortState m dom_pids ps"
+      and p_in_dom: "p \<in> dom_pids"
+     shows "wf_PortState_queues m dom_pids (portEnqueuePID ps p v)"
+  using wf_ps  \<comment> \<open>assume we start with well-formed port states\<close>  
+        p_in_dom 
+        portEnqueuePID_preserves_wf_PortState_queue
+        wf_PortState_def
+        wf_PortState_queues_def  \<comment> \<open>well-formedness definitions and associated properties\<close> 
+  by (smt (verit, best) fun_upd_apply map_get_def portEnqueuePID.simps) 
+
+(* ToDo (from John): Try getting rid of the smt in the proof above and simpifying
+  proofs above using portEnqueuePID.simps.   This seems to give the one-level
+  unfolding of function definition 
+
+  Also, if you take a look at what keeps showing up in the metis and smt proofs,
+  it is things related to map (map_get_def) and (fun_upd_apply).  It is likely
+  possible to engineer the defs/functions/lemmas so that those things don't keep
+  coming up and blocking things. *)
+
+text \<open>@{term portEnqueuePID} preserves port state well-formedness.\<close>
+
+lemma portEnqueuePID_preserves_wf_PortState: 
+ assumes wf_ps:   "wf_PortState m dom_pids ps " 
+      and p_in_dom: "p \<in> dom_pids"
+    shows "wf_PortState m dom_pids (portEnqueuePID ps p v)"
+  using wf_ps p_in_dom \<comment> \<open>assumptions\<close>
+        portEnqueuePID_preserves_wf_PortState_dom \<comment> \<open>lemmas showing subproperties of wf preserved\<close>
+        portEnqueuePID_preserves_wf_PortState_queues 
+        wf_PortState_def \<comment> \<open>definition of well-formedness\<close> 
+  by metis
+
 end
