Properties.thy
@@ -16,10 +16,10 @@ property} for thread application logic (which abstracts thread entry point code)
 The property @{term P} holds for a thread's application logic 
 if it holds for  all output variable states @{term vs'}
 and output port states @{term ps'} that satisfy the thread's Initialize
-entry point contract (@{term appInit}).\<close>
+entry point behavior (@{term appInit}).\<close>
 
-definition appInitProp :: "'a App \<Rightarrow> ('a VarState * 'a PortState \<Rightarrow> bool) \<Rightarrow> bool"
-  where "appInitProp a P \<equiv> \<forall>vs' ps'. appInit a vs' ps' \<longrightarrow> P (vs', ps')"
+definition appInitProp :: "'a AppBehavior \<Rightarrow> ('a PortState * 'a VarState  \<Rightarrow> bool) \<Rightarrow> bool"
+  where "appInitProp a P \<equiv> \<forall>ao tvo. appInit a ao tvo \<longrightarrow> P (ao, tvo)"
 
 text \<open>We introduce the notion a \emph{system initialization property}.  Currently,
 the only system features that can be ``observed'' by a system property are the variable
@@ -37,100 +37,100 @@ to thread state @{term t'}, then the @{term c}-relevant portion of the property
 holds for the variable state @{term tvar} and output application port state @{term appo}
 elements of thread state @{term t'}.\<close>
 
-definition sysInitProp :: "'a AppModel \<Rightarrow> (CompId \<Rightarrow> ('a VarState * 'a PortState \<Rightarrow> bool)) => bool"
-  where "sysInitProp am P \<equiv>
-  \<forall>c \<in> appModelCIDs am. \<forall>t t'. stepInit (appModelApp am $ c) t t' \<longrightarrow> P c (tvar t', appo t')"
+definition sysInitProp :: "'a BehaviorModel \<Rightarrow> (CompId \<Rightarrow> ('a PortState * 'a VarState  \<Rightarrow> bool)) => bool"
+  where "sysInitProp bm P \<equiv>
+  \<forall>c \<in> modelCIDs (bmmodel bm). \<forall>(t::'a ThreadState) t'. stepInit (bmbehaviors bm $ c) t t' \<longrightarrow> P c (appo t', tvar t')"
 
-text \<open>Now, we set up a verification condition @{term sysInitVC} 
-for a system initialization property @{term P}.
-We intend to show that, to verify a system initialization property @{term P} (i.e., to show
-that P holds for an app model @{term am}, it is sufficient to show that for every
-thread component @{term c} in the model, the @{term c}-relevant portion of @{term P}
-is an thread initialization property (@{term appInitProp}) for @{term c} (i.e., for
-@{term c}'s application logic).\<close>
+text \<open>Now, we set up a verification condition \<open>sysInitVC\<close> 
+for a system initialization property \<open>P\<close>.
+We intend to show that, to verify a system initialization property \<open>P\<close> (i.e., to show
+that \<open>P\<close> holds for an app model \<open>am\<close>, it is sufficient to show that for every
+thread component \<open>c\<close> in the model, the \<open>c\<close>-relevant portion of \<open>P\<close>
+is an thread initialization property (\<open>appInitProp\<close>) for \<open>c\<close> (i.e., for
+\<open>c\<close>'s application logic).\<close>
 
-definition sysInitVC :: "'a AppModel \<Rightarrow> (CompId \<Rightarrow> ('a VarState * 'a PortState \<Rightarrow> bool)) => prop"
-  where "sysInitVC am P \<equiv> 
-  (\<And>c. c \<in> appModelCIDs am \<Longrightarrow> appInitProp (appModelApp am $ c) (P c))"
+definition sysInitVC :: "'a BehaviorModel \<Rightarrow> (CompId \<Rightarrow> ('a PortState * 'a VarState  \<Rightarrow> bool)) => prop"
+  where "sysInitVC bm P \<equiv> 
+  (\<And>c. c \<in> modelCIDs (bmmodel bm) \<Longrightarrow> appInitProp (bmbehaviors bm $ c) (P c))"
 
-text \<open>The following lemma establishes that @{term sysInitVC} is a sound verification
-condition for system initialization property P: for a well-formed app model @{term am},
-if @{term sysInitVC} holds, then @{term sysInitProp} holds.\<close>
+text \<open>The following lemma establishes that \<open>sysInitVC\<close> is a sound verification
+condition for system initialization property \<open>P\<close>: for a well-formed app model \<open>am\<close>,
+if \<open>sysInitVC\<close> holds, then \<open>sysInitProp\<close> holds.\<close>
 
 lemma initSysFromApps:
-  assumes wf_am: "wf_AppModel am"
-      and vc: "\<And>c. c \<in> appModelCIDs am \<Longrightarrow> appInitProp (appModelApp am $ c) (P c)"
-    shows "sysInitProp am P"
+  assumes wf_bm: "wf_BehaviorModel (bm::'a BehaviorModel)"
+      and vc: "\<And>c. c \<in> modelCIDs (bmmodel bm) \<Longrightarrow> appInitProp (bmbehaviors bm $ c) (P c)"
+    shows "sysInitProp bm P"
 proof (simp only: sysInitProp_def; clarify)
-  fix c t t'
-  assume a1: "c \<in> appModelCIDs am"
-     and a2: "stepInit (appModelApp am $ c) t t'"
-  thus "P c (tvar t', appo t')"
+  fix c
+  fix t t'::"'a ThreadState"
+  assume a1: "c \<in> modelCIDs (bmmodel bm)"
+     and a2: "stepInit (bmbehaviors bm $ c) t t'"
+  thus "P c (appo t', tvar t')"
   proof -
-    have "appInit (appModelApp am $ c) (tvar t') (appo t')" 
-      using a2 stepInit_ruleinv[of "(appModelApp am $ c)" t t'] by blast
+    have "appInit (bmbehaviors bm $ c) (appo t') (tvar t')" 
+      using a2 stepInit_ruleinv[of "(bmbehaviors bm $ c)" t t'] by blast
     thus ?thesis
       using a1 appInitProp_def vc by blast 
   qed
 qed
 
-text \<open>The follow definition will interpret a system initialization property
-@{term P} in the context of a specific system state @{term s}.\<close>
+text \<open>The following definition will interpret a system initialization property
+\<open>P\<close> in the context of a specific system state \<open>s\<close>.\<close>
 
-definition sysAllInitProp :: "'a AppModel \<Rightarrow> 
-  (CompId \<Rightarrow> ('a VarState * 'a PortState \<Rightarrow> bool)) \<Rightarrow> 
+definition sysStateProp :: "'a BehaviorModel \<Rightarrow> 
+  (CompId \<Rightarrow> ('a PortState * 'a VarState \<Rightarrow> bool)) \<Rightarrow> 
   ('u, 'a) SystemState \<Rightarrow> bool"
-where "sysAllInitProp am P s \<equiv>
-  \<forall>c \<in> appModelCIDs am. P c (tvar (systemThread s $ c), appo (systemThread s $ c))"
+where "sysStateProp bm P s \<equiv>
+  \<forall>c \<in> modelCIDs (bmmodel bm). P c (appo (systemThread s $ c), tvar (systemThread s $ c))"
 
-definition systemAppInit where "systemAppInit am c = { (v, p) | v p. appModelInit am c v p }"
+text \<open>The following definition forms the set of all possible Initialization Entrypoint
+outputs of thread component \<open>c\<close>, where outputs are pairs of var states (\<open>tvar\<close>) \<open>v\<close> and application
+output port states (\<open>appo\<close>) \<open>ao\<close>.\<close>
 
-definition varappo where "varappo x c = 
+definition systemAppInit :: "'a BehaviorModel \<Rightarrow> CompId \<Rightarrow> ('a PortState \<times> 'a VarState ) set"
+  where "systemAppInit bm c = { (ao, tvo) | ao tvo. appInit (bmbehaviors bm $ c) ao tvo }"
+
+text \<open>The following definition projects a state to a tuple consisting of 
+thread app output port states (\<open>appo\<close>) and thread variable states (\<open>tvar\<close>) 
+-- the two thread state elements affected by thread initialisation.\<close>
+
+(* From John: it might be a good idea at some point to group in one place a collection
+    of definitions like this one that convert from a predicate view of a component behavior
+    to a tuple/relational view of component behavior *)
+
+definition appovar :: "('u, 'a) SystemState \<Rightarrow> CompId \<Rightarrow> ('a PortState \<times> 'a VarState) option"
+ where "appovar x c = 
   (if c \<in> dom (systemThread x) 
-    then Some (tvar (systemThread x $ c), appo (systemThread x $ c)) 
+    then Some (appo (systemThread x $ c), tvar (systemThread x $ c)) 
     else None)"
 
-lemma varappo_te:
+lemma appovar_te:
   assumes "c \<in> dom(systemThread x)"
-  shows "varappo (x\<lparr>systemThread := 
-    systemThread x(c \<mapsto> (systemThread x $ c)\<lparr>tvar := vs, appo := ps\<rparr>), systemExec := e\<rparr>) c = 
-    Some (vs, ps)"
+  shows "appovar (x\<lparr>systemThread := 
+    (systemThread x)(c \<mapsto> (systemThread x $ c)\<lparr>appo := ao, tvar := tvo\<rparr>), systemExec := e\<rparr>) c = 
+    Some (ao, tvo)"
 proof -
-  have h1: "tvar(systemThread x(c \<mapsto> (systemThread x $ c)\<lparr>tvar := vs, appo := ps\<rparr>) $ c) = vs"
+  have h1: "tvar((systemThread x)(c \<mapsto> (systemThread x $ c)\<lparr>appo := ao, tvar := tvo\<rparr>) $ c) = tvo"
     by simp
-  have h2: "appo(systemThread x(c \<mapsto> (systemThread x $ c)\<lparr>tvar := vs, appo := ps\<rparr>) $ c) = ps"
+  have h2: "appo((systemThread x)(c \<mapsto> (systemThread x $ c)\<lparr>appo := ao, tvar := tvo\<rparr>) $ c) = ao"
     by simp
-  show ?thesis unfolding varappo_def by simp
+  show ?thesis unfolding appovar_def by simp
 qed
 
 lemma sysInit_bw:
-  shows "\<lbrakk>stepSys am com sch x y; systemExec y = Initialize cs \<rbrakk> \<Longrightarrow> systemExec x \<noteq> Initialize []"
-proof (induction rule: stepSys.induct)
-  case (initialize c cs t)
-  then show ?case by simp
-next
-  case (switch c)
-  then show ?case by simp
-next
-  case (push c t sb it)
-  then show ?case by force
-next
-  case (pull c t sb it)
-  then show ?case by simp
-next
-  case (execute c c' a t)
-  then show ?case by simp
-qed
+  shows "\<lbrakk>stepSys bm com sc x y; systemExec y = Initialize cs \<rbrakk> \<Longrightarrow> systemExec x \<noteq> Initialize []"
+  using stepSysInit_sc_rev_ruleinv by fastforce
 
 lemma sysInit_seq_bw_neq:
-  "\<lbrakk>(stepSys am com sch)\<^sup>*\<^sup>* x y; x \<noteq> y; systemExec y = Initialize cs \<rbrakk> \<Longrightarrow> systemExec x \<noteq> Initialize []"
+  "\<lbrakk>(stepSys bm com sc)\<^sup>*\<^sup>* x y; x \<noteq> y; systemExec y = Initialize cs\<rbrakk> \<Longrightarrow> systemExec x \<noteq> Initialize []"
 proof (induction arbitrary: cs rule: rtranclp.induct)
   case (rtrancl_refl a)
   then show ?case by blast
 next
   case (rtrancl_into_rtrancl a b c)
-  have h1: "(stepSys am com sch)\<^sup>*\<^sup>* a b" using rtrancl_into_rtrancl.hyps(1) by blast
-  have h2: "stepSys am com sch b c" using rtrancl_into_rtrancl.hyps(2) by blast
+  have h1: "(stepSys bm com sc)\<^sup>*\<^sup>* a b" using rtrancl_into_rtrancl.hyps(1) by blast
+  have h2: "stepSys bm com sc b c" using rtrancl_into_rtrancl.hyps(2) by blast
   have h3: "\<And>cs. a \<noteq> b \<Longrightarrow> systemExec b = Initialize cs \<Longrightarrow> systemExec a \<noteq> Initialize []"
     using rtrancl_into_rtrancl.IH by blast
   have h4: "a \<noteq> c" by (simp add: rtrancl_into_rtrancl.prems(1))
@@ -149,7 +149,7 @@ next
 qed
 
 lemma sysInit_seq_bw_supseq:
-  "\<lbrakk>(stepSys am com sch)\<^sup>*\<^sup>* x y; systemExec y = Initialize cs \<rbrakk> \<Longrightarrow> (\<exists>as. systemExec x = Initialize (as @ cs))"
+  "\<lbrakk>(stepSys bm com sc)\<^sup>*\<^sup>* x y; systemExec y = Initialize cs \<rbrakk> \<Longrightarrow> (\<exists>as. systemExec x = Initialize (as @ cs))"
 proof (induction arbitrary: cs rule: rtranclp.induct)
   case (rtrancl_refl a)
   then show ?case by simp
@@ -160,11 +160,11 @@ next
 qed
 
 lemma sysInit_none:
-  "\<lbrakk>stepSys am com sch x y; systemExec y = Initialize cs; systemExec x = Initialize cs \<rbrakk> \<Longrightarrow> x = y"
+  "\<lbrakk>stepSys bm com sc x y; systemExec y = Initialize cs; systemExec x = Initialize cs \<rbrakk> \<Longrightarrow> x = y"
   using stepSysInit_sc_rev_ruleinv by fastforce
 
 lemma sysInit_seq_none:
-  "\<lbrakk>(stepSys am com sch)\<^sup>*\<^sup>* x y; systemExec y = Initialize cs; systemExec x = Initialize cs \<rbrakk> \<Longrightarrow> x = y"
+  "\<lbrakk>(stepSys bm com sc)\<^sup>*\<^sup>* x y; systemExec y = Initialize cs; systemExec x = Initialize cs \<rbrakk> \<Longrightarrow> x = y"
 proof (induction rule: rtranclp.induct)
   case (rtrancl_refl a)
   then show ?case by simp
@@ -177,175 +177,318 @@ next
 qed
 
 lemma sysInit_step_seq_set: 
-  "\<lbrakk> stepSys am com sch x y; 
-     isInitializing x;
-     systemExec x = Initialize (c # cs) \<rbrakk> \<Longrightarrow> varappo y \<in> { (varappo x)(c\<mapsto>v) |v. v \<in> systemAppInit am c }"
-proof (induction rule: stepSys.induct)
-  case (initialize a cs t)
-  have h1: "a = c" using initialize.hyps(2) initialize.prems(2) by fastforce
-  then obtain vs ps where 
-    h2: "varappo (x\<lparr>systemThread := systemThread x(a \<mapsto> t), systemExec := Initialize cs\<rparr>) c = Some (vs, ps)"
-    using varappo_def
-    by (metis SystemState.SystemState.select_convs(1) SystemState.SystemState.surjective 
-        SystemState.SystemState.update_convs(1) SystemState.SystemState.update_convs(5) domI fun_upd_same)
-  hence h3: "(vs, ps) \<in> systemAppInit am c" unfolding systemAppInit_def varappo_def apply clarify
-    using h1 initialize.hyps(3) stepInit_ruleinv by fastforce
-  have h4: "varappo (x\<lparr>systemThread := systemThread x(a \<mapsto> t), systemExec := Initialize cs\<rparr>) = varappo x(c \<mapsto> (vs, ps))"
-  proof
-    fix z
-    show "varappo (x\<lparr>systemThread := systemThread x(a \<mapsto> t), systemExec := Initialize cs\<rparr>) z =
-          (varappo x(c \<mapsto> (vs, ps))) z"
-    proof (cases "z = c")
-      case True
-      then show ?thesis
-        by (simp add: h2)
-    next
-      case False
-      then show ?thesis by (simp add: h1 varappo_def)
+  assumes step: "stepSys bm com sc x y"
+      and exec: "systemExec x = Initialize (c # cs)"
+    shows "appovar y \<in> { (appovar x)(c\<mapsto>v) |v. v \<in> systemAppInit bm c }"
+proof -
+  have "stepSys bm com sc x y = initStepSys bm com sc x y"
+    using stepSys_initializing exec init_init by blast
+  hence "initStepSys bm com sc x y" using step by force
+  thus ?thesis using exec
+  proof (induction rule: initStepSys.induct)
+    case (initialize s c cs t)
+    obtain ps vs where h2: "appovar (s\<lparr> systemThread := (systemThread s)(c \<mapsto> t), 
+                                        systemExec := Initialize cs\<rparr>) c = Some (ps, vs)"
+      using appovar_def domI fun_upd_same
+      by (metis SystemState.SystemState.simps(1) SystemState.SystemState.simps(9) 
+          SystemState.SystemState.surjective SystemState.SystemState.update_convs(1))
+    hence h3: "(ps, vs) \<in> systemAppInit bm c" unfolding systemAppInit_def appovar_def apply clarify
+      using initialize.hyps(3) stepInit_ruleinv by fastforce
+    have h4: "appovar (s\<lparr>systemThread := (systemThread s)(c \<mapsto> t), 
+                         systemExec := Initialize cs\<rparr>) = (appovar s)(c \<mapsto> (ps, vs))"
+    proof
+      fix z
+      show "appovar (s\<lparr>systemThread := (systemThread s)(c \<mapsto> t), systemExec := Initialize cs\<rparr>) z =
+            ((appovar s)(c \<mapsto> (ps, vs))) z"
+      proof (cases "z = c")
+        case True
+        then show ?thesis
+          by (simp add: h2)
+      next
+        case False
+        then show ?thesis by (simp add: appovar_def)
+      qed
     qed
+    then show ?case using exec h3 using initialize.hyps(2) initialize.prems by auto
+  next
+    case (switch c)
+    then show ?case by fastforce
   qed
-  show ?case using initialize.prems h2 h3 using h1 h4 by fastforce
-next
-  case (switch c)
-  then show ?case by simp
-next
-  case (push c t sb it)
-  then show ?case by simp
-next
-  case (pull c t sb it)
-  then show ?case by simp
-next
-  case (execute c c' a t)
-  then show ?case by simp
 qed
 
-lemma sysInit_step_seq: 
-  "\<lbrakk> stepSys am com sch x y; 
-     systemExec x = Initialize (c # cs) \<rbrakk> \<Longrightarrow> varappo y \<in> map_Upd_seq (systemAppInit am) {varappo x} [c]"
-proof (induction rule: stepSys.induct)
-  case (initialize a as t)
-  have h1: "a = c" using initialize.hyps(2) initialize.prems(1) by fastforce
-  have h2: "as = cs" using initialize.hyps(2) initialize.prems(1) by fastforce
-  have h3: "map_Upd_seq (systemAppInit am) {varappo x} [c] = { (varappo x)(c\<mapsto>v) |v. v \<in> systemAppInit am c }"
-    by simp
-  then show ?case apply (simp add: h3) 
-    using h1 initialize.hyps stepSys.initialize sysInit_step_seq_set by fastforce
-next
-  case (switch c)
-  then show ?case by simp
-next
-  case (push c t sb it)
-  then show ?case by simp
-next
-  case (pull c t sb it)
-  then show ?case by simp
-next
-  case (execute c c' a t)
-  then show ?case by simp
+lemma sysInit_step_seq:
+  assumes step: "stepSys bm com sc x y"
+      and exec: "systemExec x = Initialize (c # cs)"
+    shows "appovar y \<in> map_Upd_seq (systemAppInit bm) {appovar x} [c]"
+proof -
+  have "stepSys bm com sc x y = initStepSys bm com sc x y"
+    using step stepSys_initializing exec init_init by blast
+  hence h0: "initStepSys bm com sc x y" using step by force
+  thus ?thesis using exec
+  proof (induction rule: initStepSys.induct)
+    case (initialize s a as t)
+      have h1: "a = c" using initialize.hyps(2) initialize.prems(1) by fastforce
+      have h2: "as = cs" using initialize.hyps(2) initialize.prems(1) by fastforce
+      have h3: "map_Upd_seq (systemAppInit bm) {appovar s} [c] = { (appovar s)(c\<mapsto>v) |v. v \<in> systemAppInit bm c }"
+        by simp
+      show ?case
+        using step exec h0 sysInit_step_seq_set[of bm com sc s y c cs] 
+          initStepSys.initialize[of s c cs bm t] initialize.hyps(1) initialize.hyps(3)
+        apply (simp add: h1 h2 h3) 
+        using stepSys_initializing sysInit_step_seq_set
+        by (smt (verit, best) \<open>\<And>sc cm. \<lbrakk>isInitializing s; systemExec s = Initialize (c # cs); stepInit (bmbehaviors bm $ c) (systemThread s $ c) t\<rbrakk> \<Longrightarrow> initStepSys bm cm sc s (s\<lparr>systemThread := (systemThread s) (c \<mapsto> t), systemExec := Initialize cs\<rparr>)\<close> h1 h2 initialize.hyps(1) initialize.hyps(2) initialize.hyps(3) mem_Collect_eq old.prod.exhaust)
+    next
+      case (switch c) 
+        show ?case using exec switch.hyps(2) by (simp add: switch.prems)
+    qed
 qed
+
+text \<open>Lemma {sysInit\_seq} is used to prove lemma {sysInit\_init\_seq} by induction.\<close>
 
 lemma sysInit_seq:
-  "\<lbrakk> isInitializing x; stepsSys am com sch x y;
+  "\<lbrakk> stepsSys bm com sc x y;
      systemExec x = Initialize xs; systemExec y = Initialize [] \<rbrakk> \<Longrightarrow> 
-     varappo y \<in> map_Upd_seq (systemAppInit am) {varappo x} xs"
+     appovar y \<in> map_Upd_seq (systemAppInit bm) {appovar x} xs"
 proof (induction xs arbitrary: x)
   case Nil
-  then show ?case unfolding varappo_def stepsSys_def using sysInit_seq_none by fastforce
+  then show ?case unfolding appovar_def stepsSys_def using sysInit_seq_none by fastforce
 next
   case (Cons a xs)
-  obtain z where z1: "stepSys am com sch x z" 
-             and z2: "stepsSys am com sch z y"
+  have h1: "isInitializing x" by (simp add: Cons.prems(2))
+  obtain z where z1: "stepSys bm com sc x z" 
+             and z2: "stepsSys bm com sc z y"
     using Cons.prems unfolding stepsSys_def
     by (metis Exec.inject(1) converse_rtranclpE list.distinct(1))
-    have z3: "systemExec z = Initialize (xs)" using z1
-      by (metis Cons.prems(1) Cons.prems(3) stepSysInit_redsch_ruleinv)
-    have z4: "varappo z \<in> map_Upd_seq (systemAppInit am) {varappo x} [a]" 
-      using sysInit_step_seq Cons.prems(3) z1 by fastforce
+    have z3: "systemExec z = Initialize (xs)" using z1 h1 Cons.prems(2) stepSysInit_redsch_ruleinv by blast
+    have z4: "appovar z \<in> map_Upd_seq (systemAppInit bm) {appovar x} [a]" 
+      using sysInit_step_seq Cons.prems(3) z1 Cons.prems(2) by blast
   show ?case using Cons.prems Cons.IH[of z] z1 z2 z3 z4
-    by (metis (no_types, opaque_lifting) append_Cons append_Nil map_Upd_seq_comp_in stepSysInit_initInv_ruleinv)
+    by (metis (no_types, opaque_lifting) append_Cons append_Nil map_Upd_seq_comp_in)
 qed
 
+text \<open>Lemma {sysInit\_init\_seq} shows that the system initialisations can also be expressed by 
+means of the recursive function \<open>map_Upd_seq\<close>.\<close>
+
 lemma sysInit_init_seq:
-  assumes init: "isInitializing x"
-      and steps: "stepsSys am com sch x y"
-      and exec_x: "systemExec x = Initialize (scheduleInit sch)"
+  assumes steps: "stepsSys bm com sc x y"
+      and exec_x: "systemExec x = Initialize (scheduleInit sc)"
       and exec_y: "systemExec y = Initialize []"
-    shows "varappo y \<in> map_Upd_seq (systemAppInit am) {varappo x} (scheduleInit sch)"
+    shows "appovar y \<in> map_Upd_seq (systemAppInit bm) {appovar x} (scheduleInit sc)"
   using assms by (simp add: sysInit_seq)
 
+text \<open>Lemma {sysInit\_init\_merge} shows that the order of initialisations does not matter.\<close>
+
 lemma sysInit_init_merge:
-  assumes wf_am: "wf_AppModel am"
-      and wf_sch: "wf_SystemSchedule (appModel am) sch"
-      and init: "isInitializing x"
-      and steps: "stepsSys am com sch x y"
-      and exec_x: "systemExec x = Initialize (scheduleInit sch)"
+  assumes wf_bm: "wf_BehaviorModel bm"
+      and wf_sch: "wf_SystemSchedule (bmmodel bm) sc"
+      and steps: "stepsSys bm com sc x y"
+      and exec_x: "systemExec x = Initialize (scheduleInit sc)"
       and exec_y: "systemExec y = Initialize []"
-    shows "varappo y \<in> 
-    {varappo x} ** {\<Uplus>\<^sub>m set ms |ms. map_seq_in ms (map (maps_of (systemAppInit am)) (scheduleInit sch))}"
+    shows "appovar y \<in> 
+    {appovar x} ** {\<Uplus>\<^sub>m set ms |ms. map_seq_in ms (map (maps_of (systemAppInit bm)) (scheduleInit sc))}"
 proof -
-  have h1: "card (set (scheduleInit sch)) = length (scheduleInit sch)"
+  have h0: "isInitializing x" by (simp add: exec_x)
+  have h1: "card (set (scheduleInit sc)) = length (scheduleInit sc)"
     using wf_sch unfolding wf_SystemSchedule_def by simp
-  have h2: "\<forall>c \<in> dom (modelCompDescrs (appModel am)). (\<exists>ws qs. (appModelInit am c) ws qs)"
-    using wf_am unfolding wf_AppModel_def wf_App_def wf_CIDAppCIDAPP_def wf_CIDApp_def by simp
-  hence h3: "\<forall>x \<in> set (scheduleInit sch). systemAppInit am x \<noteq> {}"
+  have h2: "\<forall>c \<in> modelCIDs (bmmodel bm). (\<exists>ws qs. appInit (bmbehaviors bm $ c) ws qs)"
+    using wf_bm unfolding wf_BehaviorModel_def wf_AppBehaviors_def wf_AppBehavior_def wf_InitBehavior_Inhabited_def by auto
+  hence h3: "\<forall>x \<in> set (scheduleInit sc). systemAppInit bm x \<noteq> {}"
     using wf_sch unfolding wf_SystemSchedule_def systemAppInit_def by simp
   show ?thesis 
-    using exec_x exec_y init steps h1 h3 
-      sysInit_init_seq[of x am com sch y] 
-      map_Upd_Merge[of "(scheduleInit sch)" "(systemAppInit am)" "{varappo x}"]
+    using exec_x exec_y h0 steps h1 h3 
+      sysInit_init_seq[of bm com sc x y] 
+      map_Upd_Merge[of "(scheduleInit sc)" "(systemAppInit bm)" "{appovar x}"]
     by blast
 qed
 
-lemma sysInit_init_prop:
-  assumes wf_am: "wf_AppModel am"
-      and wf_sch: "wf_SystemSchedule (appModel am) sch"
-      and wf_state: "dom (systemThread x) \<subseteq> appModelCIDs am" (* to be included in wf_Thread *)
-      and init: "isInitializing x"
-      and exec_x: "systemExec x = Initialize (scheduleInit sch)"
+text \<open>Lemma {sysInit\_init\_prop} describes that after initialisation in any well-formed order
+all initialisation properties hold, given that the verification properties {vc} hold.
+No assumption is made concerning the executed initialisations 
+except that all of them must have been executed. This can also be seen as a consequence of lemma
+{sysInit\_init\_merge} above that shows that any order of initialisations can be replaced by the
+simultaneous execution of all initialisations.
+
+The proof uses the following strategy.
+Given the sequence of app initialisations \<open>scheduleInit sc\<close>, 
+executing them with \<open>stepsSys\<close> \ldots \<open>y\<close>,
+the property \<open>sysStateProp\<close> \ldots \<open>P y\<close>.
+In order to show this, we first show that the effect of \<open>stepsSys\<close> \ldots \<open>y\<close> can be simulated
+by \<open>appovar y \<in> map_Upd_seq\<close> \ldots\enspace. 
+This is done by induction, replacing \<open>scheduleInit sc\<close> by 
+a variable \<open>xs\<close>, in lemma {sysInit\_seq}.
+The term \<open>appovar y \<in> map_Upd_seq\<close> \ldots can be shown to equal 
+\<open>appovar y \<in> {\<Uplus>\<^sub>m set ms |ms. map_seq_in ms\<close> \ldots \<open>(scheduleInit sc))}\<close>
+using lemmas {map\_Upd\_Merge} and {map\_seq\_merge\_eq}.
+This establishes that all initial states hold simultaneously.
+Quantifying over the components \<open>c\<close> and using {vc}, we prove \<open>sysStateProp\<close> \ldots \<open>P y\<close>.
+\<close>
+
+lemma sysInit_state_prop:
+  assumes wf_bm: "wf_BehaviorModel bm"
+      and wf_sch: "wf_SystemSchedule (bmmodel bm) sc"
+      and wf_state: "wf_SystemState (bmmodel bm) x"
+      and exec_x: "systemExec x = Initialize (scheduleInit sc)"
       and exec_y: "systemExec y = Initialize []"
-      and steps: "stepsSys am com sch x y"
-      and vc: "\<And>c. c \<in> appModelCIDs am \<Longrightarrow> appInitProp (appModelApp am $ c) (P c)"
-    shows "sysAllInitProp am P y"
+      and steps: "stepsSys bm com sc x y"
+      and vc: "\<And>c. c \<in> modelCIDs (bmmodel bm) \<Longrightarrow> appInitProp (bmbehaviors bm $ c) (P c)"
+    shows "sysStateProp bm P y"
 proof -
-  have h0: "dom (varappo x) \<subseteq> appModelCIDs am" using wf_state unfolding varappo_def dom_def by auto
-  have h1: "varappo y \<in> {varappo x} ** {\<Uplus>\<^sub>m set ms |ms. map_seq_in ms (map (maps_of (systemAppInit am)) (scheduleInit sch))}"
-    using exec_x exec_y init steps sysInit_init_merge wf_am wf_sch by blast
-  have g0: "\<forall>m \<in> {\<Uplus>\<^sub>m set ms |ms. map_seq_in ms (map (maps_of (systemAppInit am)) (scheduleInit sch))}. dom (varappo x) \<subseteq> dom m"
+  have i0: "isInitializing x" by (simp add: exec_x)
+  have h0: "dom (appovar x) \<subseteq> modelCIDs (bmmodel bm)" 
+    using wf_state unfolding appovar_def dom_def wf_SystemState_def by auto
+  have h1: "appovar y \<in> {appovar x} ** {\<Uplus>\<^sub>m set ms |ms. map_seq_in ms (map (maps_of (systemAppInit bm)) (scheduleInit sc))}"
+    using exec_x exec_y i0 steps sysInit_init_merge wf_bm wf_sch by blast
+  have g0: "\<forall>m \<in> {\<Uplus>\<^sub>m set ms |ms. map_seq_in ms (map (maps_of (systemAppInit bm)) (scheduleInit sc))}. dom (appovar x) \<subseteq> dom m"
     using h0 wf_sch unfolding wf_SystemSchedule_def
-    by (smt (verit, best) CollectD appModelCIDs.elims appModelCompDescrs.simps map_seq_merge_eq)
-  have g1: "varappo y \<in> {\<Uplus>\<^sub>m set ms |ms. map_seq_in ms (map (maps_of (systemAppInit am)) (scheduleInit sch))}"
+     by (smt (verit) CollectD map_seq_merge_eq modelCIDs.simps)
+  have g1: "appovar y \<in> {\<Uplus>\<^sub>m set ms |ms. map_seq_in ms (map (maps_of (systemAppInit bm)) (scheduleInit sc))}"
     by (metis (no_types, lifting) g0 h1 map_Add_extend singleton_iff)
-  hence h2: "\<And>c. c \<in> appModelCIDs am \<Longrightarrow> varappo y $ c \<in> systemAppInit am c"
+  hence h2: "\<And>c. c \<in> modelCIDs (bmmodel bm) \<Longrightarrow> appovar y $ c \<in> systemAppInit bm c"
   proof -
     fix c
-    assume a1: "c \<in> appModelCIDs am"
-    have "card (set (scheduleInit sch)) = length (scheduleInit sch)"
+    assume a1: "c \<in> modelCIDs (bmmodel bm)"
+    have "card (set (scheduleInit sc)) = length (scheduleInit sc)"
       using wf_SystemSchedule_def wf_sch by presburger
-    show "varappo y $ c \<in> systemAppInit am c"
+    show "appovar y $ c \<in> systemAppInit bm c"
       using a1 g1 map_seq_merge_el wf_SystemSchedule_def wf_sch by fastforce
   qed
-  hence h3: "\<forall>c \<in> appModelCIDs am. (tvar (systemThread y $ c), appo (systemThread y $ c)) \<in> systemAppInit am c"
-    using g1 wf_sch unfolding wf_SystemSchedule_def
-    by (smt (verit, ccfv_SIG) appModelCIDs.elims appModelCompDescrs.simps domIff map_seq_dom_dep 
-        map_some_val_given mem_Collect_eq varappo_def)
-  have h4: "\<forall>c \<in> appModelCIDs am. P c (tvar (systemThread y $ c), appo (systemThread y $ c))"
-    by (smt (verit) appInitProp_def appModelInit.simps h3 mem_Collect_eq systemAppInit_def vc)
-  thus ?thesis using sysAllInitProp_def by blast
+  hence h3: "\<forall>c \<in> modelCIDs (bmmodel bm). 
+               (appo (systemThread y $ c), tvar (systemThread y $ c)) \<in> systemAppInit bm c"
+    using g1 wf_sch wf_state unfolding wf_SystemSchedule_def
+    by (smt (verit, best) CollectD domIff map_seq_merge_eq map_some_val_given modelCIDs.simps appovar_def)
+  have h4: "\<forall>c \<in> modelCIDs (bmmodel bm). P c (appo (systemThread y $ c), tvar (systemThread y $ c))"
+    by (smt (verit, best) appInitProp_def h3 mem_Collect_eq systemAppInit_def vc)
+  thus ?thesis using sysStateProp_def by blast 
 qed
 
-definition sysAppInvProp where "sysAppInvProp cids P I \<equiv> \<forall>c \<in> cids. \<forall>x p. P c (x, p) \<longrightarrow> I c x"
+definition sysAppInvProp ::   "CompIds 
+                            \<Rightarrow> (CompId \<Rightarrow> ('a PortState \<times> 'a VarState \<Rightarrow> bool))
+                            \<Rightarrow> (CompId \<Rightarrow> 'a VarState \<Rightarrow> bool)
+                            \<Rightarrow> bool"
+  where "sysAppInvProp cids P I \<equiv> \<forall>c \<in> cids. \<forall>ao tvo. P c (ao, tvo) \<longrightarrow> I c tvo"
 
 (* App computation invariant I on local variables and output port properties P. *)
 (* All other port properties must be guaranteed on system level. *)
 (* Also system-wide invariants must be dealt with globally, assume substrate properties. *)
-definition appInvProp where "appInvProp a I P \<equiv> 
-  \<forall>x x' d p p'. I x \<and> appCompute a x p d x' p' \<longrightarrow> I x' \<and> P (x', p')"
+definition appInvProp ::   
+   " 'a AppBehavior \<Rightarrow> 
+    ('a VarState \<Rightarrow> bool) \<Rightarrow>  \<comment> \<open>Invariant on variable states\<close> 
+    (('a PortState \<times> 'a VarState) \<Rightarrow> bool) \<Rightarrow> 
+    bool"
+  where "appInvProp a I P \<equiv> 
+   \<forall>ai tvi d ao tvo. (I tvi) \<and> ((appCompute a) ai tvi d ao tvo) \<longrightarrow> (I tvo) \<and> P (ao, tvo)"
 
-definition sysInvProp where "sysInvProp am sch I P \<equiv> 
-  \<forall>c \<in> appModelCIDs am. 
-    \<forall>t t'. I c (tvar t) \<and> 
-      stepThread (computeDispatchStatus (appModel am) c) (appModelPortKind am) (appModelApp am $ c) sch t t' 
-      \<longrightarrow> I c (tvar t) \<and> P c (tvar t, appo t)"
+definition sysInvProp ::
+  "'a BehaviorModel
+     \<Rightarrow> ScheduleState \<times> ScheduleState
+        \<Rightarrow> (CompId \<Rightarrow> 'a VarState \<Rightarrow> bool)
+           \<Rightarrow> (CompId \<Rightarrow> 'a PortState \<times> 'a VarState \<Rightarrow> bool) 
+             \<Rightarrow> bool"
+  where "sysInvProp bm sc I P \<equiv>
+  \<forall>c \<in>  modelCIDs (bmmodel bm). 
+    \<forall>(t:: 'a ThreadState) t'. I c (tvar t) \<and> 
+      stepThread (computeDispatchStatus (bmmodel bm) c) 
+                 (kindPID (bmmodel bm)) 
+                 ((bmbehaviors bm) $ c) 
+                 sc 
+                 t t' 
+      \<longrightarrow> I c (tvar t) \<and> P c (appo t, tvar t)"
+
+lemma "\<lbrakk> (stepSys am cm sc)\<^sup>*\<^sup>* s s'; isInitializing s' \<rbrakk> \<Longrightarrow> (initStepSys am cm sc)\<^sup>*\<^sup>* s s'"
+proof (induction rule: rtranclp.induct)
+  case (rtrancl_refl a)
+  then show ?case by simp
+next
+  case (rtrancl_into_rtrancl a b c)
+  have h: "isInitializing b"
+    using rtrancl_into_rtrancl.hyps(2) rtrancl_into_rtrancl.prems stepSys_initializing_back by blast
+  hence "(initStepSys am cm sc)\<^sup>*\<^sup>* a b" using rtrancl_into_rtrancl.IH by blast
+  then show ?case by (meson h rtrancl_into_rtrancl.hyps(2) rtranclp.simps stepSys_initializing)
+qed
+
+lemma "\<lbrakk> (stepSys am cm sc)\<^sup>*\<^sup>* s s'; isComputing s \<rbrakk> \<Longrightarrow> (computeStepSys am cm sc)\<^sup>*\<^sup>* s s'"
+proof (induction rule: rtranclp.induct)
+  case (rtrancl_refl a)
+  then show ?case by blast
+next
+  case (rtrancl_into_rtrancl a b c)
+  have h: "(computeStepSys am cm sc)\<^sup>*\<^sup>* a b" 
+    using rtrancl_into_rtrancl.IH rtrancl_into_rtrancl.prems by blast
+  have "isComputing b"
+    using rtrancl_into_rtrancl.hyps(1) rtrancl_into_rtrancl.prems 
+    apply simp by (metis Exec.distinct(1) Exec.exhaust sysInit_seq_bw_supseq)
+  then show ?case using initialize_not_compute
+    by (meson h rtrancl_into_rtrancl.hyps(2) rtranclp.rtrancl_into_rtrancl stepSys_def)
+qed
+
+lemma stepSysDcmpL: "(stepSys am cm sc)\<^sup>*\<^sup>* s s' \<Longrightarrow> ((initStepSys am cm sc)\<^sup>*\<^sup>* OO (computeStepSys am cm sc)\<^sup>*\<^sup>*) s s'"
+proof (induction rule: rtranclp.induct)
+  case (rtrancl_refl a)
+  then show ?case by blast
+next
+  case (rtrancl_into_rtrancl a b c)
+  obtain x where x1: "(initStepSys am cm sc)\<^sup>*\<^sup>* a x" and x2: "(computeStepSys am cm sc)\<^sup>*\<^sup>* x b"
+    using rtrancl_into_rtrancl.IH by blast
+  then show ?case
+  proof (cases "x = b")
+    case True
+    then show ?thesis by (metis relcomppI rtrancl_into_rtrancl.hyps(2) rtranclp.simps stepSys_def x1)
+  next
+    case False
+    have "isComputing x" using False compute_not_initialize
+      by (metis Exec.exhaust converse_rtranclpE init_init isComputing.elims(3) x2)
+    hence "computeStepSys am cm sc b c" 
+      using stepSys_def stepSys_initializing_back x2 compute_not_initialize initialize_not_compute
+      by (metis Exec.exhaust isComputing.simps isInitializing.elims(3) rtrancl_into_rtrancl.hyps(2) rtranclp.cases)
+    then show ?thesis using x1 x2 by auto
+  qed
+qed
+
+lemma stepSysDcmpR:
+  assumes "((initStepSys am cm sc)\<^sup>*\<^sup>* OO (computeStepSys am cm sc)\<^sup>*\<^sup>*) s s'"
+  shows "(stepSys am cm sc)\<^sup>*\<^sup>* s s'"
+proof -
+  have "((stepSys am cm sc)\<^sup>*\<^sup>* OO (stepSys am cm sc)\<^sup>*\<^sup>*) s s'"
+    using stepSys_init_rtranclp stepSys_compute_rtranclp using assms by blast
+  thus ?thesis by force
+qed
+
+lemma stepSysDcmp: "(stepSys am cm sc)\<^sup>*\<^sup>* = (initStepSys am cm sc)\<^sup>*\<^sup>* OO (computeStepSys am cm sc)\<^sup>*\<^sup>*"
+proof -
+  have "\<And>s s'. (stepSys am cm sc)\<^sup>*\<^sup>* s s' = ((initStepSys am cm sc)\<^sup>*\<^sup>* OO (computeStepSys am cm sc)\<^sup>*\<^sup>*) s s'"
+    using stepSysDcmpL stepSysDcmpR by metis
+  thus ?thesis by presburger
+qed
+
+lemma sysBehaviorDcmp:
+  assumes wf_bm: "wf_BehaviorModel bm"
+      and wf_sch: "wf_SystemSchedule (bmmodel bm) sc"
+      and init: "initSys bm sc x"
+      and steps: "stepsSys bm cm sc x z"
+      and comp: "isComputing z"
+      and vc: "\<And>c. c \<in> modelCIDs (bmmodel bm) \<Longrightarrow> appInitProp (bmbehaviors bm $ c) (P c)"
+    shows "\<exists>y. initStepsSys bm cm sc x y \<and> sysStateProp bm P y \<and> computeStepsSys bm cm sc y z"
+proof -
+  obtain y where y1: "(initStepSys bm cm sc)\<^sup>*\<^sup>* x y" and y2: "(computeStepSys bm cm sc)\<^sup>*\<^sup>* y z"
+    by (metis pick_middlep stepSysDcmpL steps stepsSys_def)
+  have h1: "isInitializing x" using init initSys_def by auto
+  have h2: "isComputing y" using y2 comp compute_compute compute_not_initialize
+    by (metis Exec.exhaust converse_rtranclpE isInitializing.simps)
+  have "x \<noteq> y" using compute_not_init h1 h2 by blast
+  then obtain y' where y3: "(initStepSys bm cm sc)\<^sup>*\<^sup>* x y'" and y4: "initStepSys bm cm sc y' y"
+    by (metis rtranclp.cases y1)
+  have h3: "systemExec y' = Initialize []"
+    by (meson compute_not_init h2 initStepSys.cases stepSysInit_initInv_ruleinv stepSys_init y4)
+  have h4: "systemExec x = Initialize (scheduleInit sc)" using init initSys_def by blast
+  have h5: "wf_SystemState (bmmodel bm) x" using init initSys_def by blast
+  have "sysStateProp bm P y'"
+    using sysInit_state_prop[of bm sc x y' cm P] using wf_bm wf_sch using h3 h4 vc y3 h5 
+    by (metis stepSys_init_rtranclp stepsSys_def)
+  hence "sysStateProp bm P y"
+    using y4 h2 stepSys_init[of bm cm sc y' y] unfolding sysStateProp_def apply clarify
+    using initStepSys.simps stepSysInit_initInv_ruleinv by fastforce
+  then show ?thesis by (metis computeStepsSys_def initStepsSys_def y1 y2)
+qed
 
 (*
 lemma sysThreadInv:
@@ -353,7 +496,7 @@ lemma sysThreadInv:
       and valid: "c \<in> appModelCIDs am"
       and isat: "I c (tvar x)"
       and inv: "appInvProp (appModelApp am $ c) (I c) (P c)"
-    shows "sysInvProp am sch I P"
+    shows "sysInvProp am sc I P"
   using wf_am unfolding wf_AppModel_def wf_CIDAppCIDAPP_def wf_CIDApp_def
   by blast
 
@@ -361,8 +504,8 @@ lemma sysThreadInv:
 lemma sysThreadInv1:
   assumes wf_am: "wf_AppModel am"
       and vc: "\<And>c. \<lbrakk>c \<in> appModelCIDs am; I c (tvar x)\<rbrakk> \<Longrightarrow> appInvProp (appModelApp am $ c) (I c) (P c)"
-      and step: "stepComp (computeDispatchStatus (appModel am) c) (appModelApp am $ c) sch x y"
-    shows "sysInvProp am sch I P"
+      and step: "stepComp (computeDispatchStatus (appModel am) c) (appModelApp am $ c) sc x y"
+    shows "sysInvProp am sc I P"
   using wf_am unfolding wf_AppModel_def wf_CIDAppCIDAPP_def wf_CIDApp_def
   by blast
 *)
