RTS.thy
@@ -1,0 +1,53 @@
+theory RTS
+  imports ThreadState
+begin
+
+fun receiveInputSrcOld where
+  "receiveInputSrcOld pki ps src dst p = (if p \<in> ps then 
+  (case pki p of
+    Data \<Rightarrow> Some (clear (src $ p))
+  | Event \<Rightarrow> Some (tail (src $ p))
+  | EventData \<Rightarrow> Some (clear (src $ p))
+  )
+  else None)"
+
+fun receiveInputSrc where
+  "receiveInputSrc pki ps src dst p = (if p \<in> ps then 
+  (case pki p of
+    Data \<Rightarrow> Some (src $ p)
+  | Event \<Rightarrow> Some (tail (src $ p))
+  | EventData \<Rightarrow> Some (tail (src $ p))
+  )
+  else None)"
+
+fun receiveInputDstOld where
+  "receiveInputDstOld pki ps src dst p = (if p \<in> ps then
+  (case pki p of
+    Data \<Rightarrow> Some (src $ p )
+  | Event \<Rightarrow> Some (setBuffer (dst $ p) [head (src $ p)] )
+  | EventData \<Rightarrow> Some (clear (dst $ p))
+  )
+  else None)"
+
+fun receiveInputDst where
+  "receiveInputDst pki ps src dst p = (if p \<in> ps then
+  (case pki p of
+    Data \<Rightarrow> Some (src $ p )
+  | Event \<Rightarrow> Some (setBuffer (dst $ p) [head (src $ p)] )
+  | EventData \<Rightarrow> Some (setBuffer (dst $ p) [head (src $ p)])
+  )
+  else None)"
+
+inductive receiveInput for pki :: "PortId \<Rightarrow> PortKind"
+                      and ps :: "PortIds"
+                      and src :: "'a PortState"
+                      and dst :: "'a PortState" where
+  default: "receiveInput pki ps src dst 
+              (receiveInputSrc pki ps src dst) 
+              (receiveInputDst pki ps src dst)"
+
+inductive sendOutput for src :: "'a PortState"
+                      and dst :: "'a PortState" where
+  default: "sendOutput src dst (clearAll (dom src) src) src"
+
+end
